natural_type_environment.v
@@ -49,6 +49,7 @@ Definition natural_size_of (Γ : env Ti) : type Ti → nat :=
 
 Instance natural_env : Env Ti := {
   size_of := natural_size_of;
+  align_of := natural_align_of;
   field_sizes Γ τs :=
     natural_field_sizes (natural_size_of Γ) Γ (natural_fields_align Γ τs) 0 τs;
   alloc_can_fail := alloc_can_fail
@@ -74,23 +75,25 @@ Proof.
   intros fcompound rec1 rec2 c s τs _.
   unfold fcompound. induction 1; simpl; auto using f_equal.
 Qed.
-Lemma natural_align_of_base Γ τb :
-  natural_align_of Γ (baseT τb) = align_base τb.
+Lemma natural_align_of_base Γ τb : align_of Γ (baseT τb) = align_base τb.
 Proof. done. Qed.
-Lemma natural_align_of_array Γ τ n :
-  natural_align_of Γ (τ.[n]) = natural_align_of Γ τ.
-Proof. unfold natural_align_of. by rewrite type_iter_array. Qed.
+Lemma natural_align_of_array Γ τ n : align_of Γ (τ.[n]) = align_of Γ τ.
+Proof.
+  unfold align_of; simpl; unfold natural_align_of. by rewrite type_iter_array.
+Qed.
 Lemma natural_align_of_compound Γ c s τs :
   ✓ Γ → Γ !! s = Some τs →
-  natural_align_of Γ (compoundT{c} s) = natural_fields_align Γ τs.
+  align_of Γ (compoundT{c} s) = natural_fields_align Γ τs.
 Proof.
-  intros. unfold natural_align_of. by rewrite type_iter_compound by eauto
+  intros. unfold align_of; simpl; unfold natural_align_of.
+  by rewrite type_iter_compound by eauto
     using natural_align_of_compound_proper with typeclass_instances.
 Qed.
-Lemma natural_align_weaken Γ1 Γ2 τ :
-  ✓ Γ1 → ✓{Γ1} τ → Γ1 ⊆ Γ2 → natural_align_of Γ1 τ = natural_align_of Γ2 τ.
+Lemma natural_align_of_weaken Γ1 Γ2 τ :
+  ✓ Γ1 → ✓{Γ1} τ → Γ1 ⊆ Γ2 → align_of Γ1 τ = align_of Γ2 τ.
 Proof.
-  intros. unfold natural_align_of. apply type_iter_weaken; eauto
+  intros. unfold align_of; simpl; unfold natural_align_of.
+  apply type_iter_weaken; eauto
     using natural_align_of_compound_proper with typeclass_instances.
 Qed.
 Lemma natural_fields_align_weaken Γ1 Γ2 τs :
@@ -98,7 +101,7 @@ Lemma natural_fields_align_weaken Γ1 Γ2 τs :
   natural_fields_align Γ1 τs = natural_fields_align Γ2 τs.
 Proof.
   intros ? Hτs ?. unfold natural_fields_align.
-  induction Hτs; simpl; auto using natural_align_weaken.
+  induction Hτs; simpl; auto using natural_align_of_weaken.
 Qed.
 Lemma natural_field_sizes_weaken rec1 rec2 Γ1 Γ2 whole_align pos τs :
   ✓ Γ1 → Γ1 ⊆ Γ2 → ✓{Γ1}* τs → Forall (λ τ, rec1 τ = rec2 τ) τs →
@@ -108,7 +111,7 @@ Proof.
   intros ?? Hτs Hrec. revert pos Hτs.
   induction Hrec as [|τ τs Hτ ? IH]; intros; decompose_Forall; simpl; auto.
   rewrite Hτ, IH by done. destruct τs as [|τ2 τs]; simpl; [done|].
-  decompose_Forall. by erewrite natural_align_weaken by eauto.
+  decompose_Forall. by erewrite natural_align_of_weaken by eauto.
 Qed.
 
 Lemma natural_size_of_compound_proper Γ1 Γ2 rec1 rec2 c s τs :
@@ -134,6 +137,8 @@ Lemma natural_size_of_base Γ τb :
     | voidT => 1 | intT τi => rank_size (rank τi) | τp.* => ptr_size τp
     end%BT.
 Proof. done. Qed.
+Lemma natural_size_of_array Γ τ n : size_of Γ (τ.[n]) = n * size_of Γ τ.
+Proof. unfold size_of; simpl. by apply type_iter_array. Qed.
 Lemma natural_size_of_compound Γ c s τs :
   ✓ Γ → Γ !! s = Some τs → size_of Γ (compoundT{c} s) =
     match c with
@@ -154,6 +159,16 @@ Proof.
   apply type_iter_weaken;
     eauto using natural_size_of_compound_proper with typeclass_instances.
 Qed.
+Lemma natural_align_ne_0 Γ τ : ✓ Γ → ✓{Γ} τ → align_of Γ τ ≠ 0.
+Proof.
+  intros HΓ. revert τ. refine (type_env_ind _ HΓ _ _ _ _).
+  * intros τb _; rewrite natural_align_of_base; destruct τb;
+      rewrite ?align_void; eauto using Nat_divide_ne_0, rank_size_ne_0.
+  * intros. by rewrite natural_align_of_array.
+  * intros c s τs Hs _ IH _. erewrite natural_align_of_compound by eauto.
+    clear Hs. unfold natural_fields_align.
+    induction IH; csimpl; rewrite ?Nat.lcm_eq_0; naive_solver.
+Qed.
 
 Instance natural_env_spec: EnvSpec Ti.
 Proof.
@@ -162,8 +177,7 @@ Proof.
   * intros ??. apply ptr_size_ne_0.
   * done.
   * done.
-  * intros ???. unfold size_of; simpl. unfold natural_size_of.
-    by rewrite type_iter_array.
+  * by apply natural_size_of_array.
   * intros Γ s τs ??. by erewrite natural_size_of_compound by eauto.
   * intros Γ τs ?. unfold field_sizes; simpl.
     change natural_size_of with size_of.
@@ -174,60 +188,52 @@ Proof.
       size_of Γ τ ≤ foldr max 1 (size_of Γ <$> τs)); [|simpl; auto with lia].
     clear Hτs. induction τs; csimpl; constructor; [lia|].
     eapply Forall_impl; eauto with lia.
+  * intros Γ τ n. by rewrite natural_align_of_array.
+  * intros Γ c s τs i τ ? Hs Hi. erewrite natural_align_of_compound by eauto.
+    clear Hs. revert i τ Hi. unfold natural_fields_align.
+    induction τs; intros [|?] ??; simplify_equality';
+      eauto 3 using Nat.divide_trans, Nat.divide_lcm_r, Nat.divide_lcm_l.
+  * intros Γ τ HΓ. revert τ. unfold size_of; simpl.
+    refine (type_env_ind _ HΓ _ _ _ _).
+    + intros τb. rewrite natural_align_of_base, natural_size_of_base.
+      destruct 1; auto. by rewrite align_void.
+    + intros τ n ? ? _. rewrite natural_align_of_array, natural_size_of_array.
+      by apply Nat.divide_mul_r.
+    + intros c s τs Hs Hτs IH Hlen.
+      erewrite natural_align_of_compound, natural_size_of_compound by eauto.
+      assert (natural_fields_align Γ τs ≠ 0) as Hne_0.
+      { clear Hs Hlen. unfold natural_fields_align.
+        induction IH as [|τ τs IHτ ? IH]; decompose_Forall; simpl; [done|].
+        rewrite Nat.lcm_eq_0; intros [|?]; [|by destruct IH].
+        by apply natural_align_ne_0. }
+      destruct c; [|by apply natural_padding_divide].
+      clear Hs Hτs IH. unfold field_sizes; simpl. revert Hne_0.
+      generalize (natural_fields_align Γ τs); intros whole_align ?.
+      rewrite <-(Nat.add_0_l (sum_list _)). generalize 0.
+      induction τs as [|τ1 τs IH]; intros pos; simpl; [done|].
+      rewrite (Nat.add_assoc pos), (Nat.add_comm pos).
+      destruct τs as [|τ2 τs]; [simpl|by apply IH].
+      rewrite Nat.add_0_r, <-Nat.add_assoc, (Nat.add_comm _ pos),
+        Nat.add_assoc; auto using natural_padding_divide.
+  * intros Γ τs i τ ? Hτs. revert i.
+    cut (∀ whole_align i pos, τs !! i = Some τ →
+      (default whole_align (head τs) (natural_align_of Γ) | pos) →
+      (natural_align_of Γ τ | pos + sum_list (take i
+         (natural_field_sizes (natural_size_of Γ) Γ whole_align pos τs)))).
+    { intros help i ?. rewrite <-(Nat.add_0_l (field_offset _ _ _)).
+      apply help; auto using Nat.divide_0_r. }
+    intros whole_align. induction Hτs as [|τ' τs Hτ Hτs IH];
+      intros [|i] pos al ?; simplify_equality'.
+    { rewrite Nat.add_0_r. auto using Nat.divide_0_r. }
+    rewrite Nat.add_assoc, (Nat.add_comm pos). apply IH; auto.
+    clear IH. destruct Hτs as [|τ2 τs]; simplify_list_equality.
+    rewrite <-Nat.add_assoc, (Nat.add_comm _ pos), Nat.add_assoc.
+    by apply natural_padding_divide, natural_align_ne_0.
   * apply natural_size_of_weaken.
+  * apply natural_align_of_weaken.
   * intros Γ1 Γ2 τs ? Hτs ?. unfold field_sizes; simpl.
     assert (Forall (λ τ, size_of Γ1 τ = size_of Γ2 τ) τs).
     { induction Hτs; constructor; auto using natural_size_of_weaken. }
-    by erewrite natural_field_sizes_weaken,
-      natural_fields_align_weaken by eauto.
-Qed.
-
-Lemma natural_align_of_divide Γ τ :
-  ✓ Γ → ✓{Γ} τ → (natural_align_of Γ τ | size_of Γ τ).
-Proof.
-  intros HΓ. revert τ. refine (type_env_ind _ HΓ _ _ _ _).
-  * intros τb. rewrite natural_align_of_base, natural_size_of_base.
-    destruct 1; auto. by rewrite align_void.
-  * intros τ n ? ? _. rewrite natural_align_of_array, size_of_array.
-    by apply Nat.divide_mul_r.
-  * intros c s τs Hs Hτs IH Hlen.
-    erewrite natural_align_of_compound, natural_size_of_compound by eauto.
-    assert (natural_fields_align Γ τs ≠ 0) as Hne_0.
-    { clear Hs Hlen. unfold natural_fields_align.
-      induction IH as [|τ τs IHτ ? IH]; decompose_Forall; simpl; [done|].
-      rewrite Nat.lcm_eq_0; intros [|?]; [|by destruct IH].
-      apply Nat_divide_ne_0 with (size_of Γ τ); auto using size_of_ne_0. }
-    destruct c; [|by apply natural_padding_divide].
-    clear Hs Hτs IH. unfold field_sizes; simpl. revert Hne_0.
-    generalize (natural_fields_align Γ τs); intros whole_align ?.
-    rewrite <-(Nat.add_0_l (sum_list _)). generalize 0.
-    induction τs as [|τ1 τs IH]; intros pos; simpl; [done|].
-    rewrite (Nat.add_assoc pos), (Nat.add_comm pos).
-    destruct τs as [|τ2 τs]; [simpl|by apply IH].
-    rewrite Nat.add_0_r, <-Nat.add_assoc, (Nat.add_comm _ pos),
-      Nat.add_assoc; auto using natural_padding_divide.
-Qed.
-Lemma natural_align_ne_0 Γ τ : ✓ Γ → ✓{Γ} τ → natural_align_of Γ τ ≠ 0.
-Proof.
-  intros. apply Nat_divide_ne_0 with (size_of Γ τ); auto
-    using natural_align_of_divide, size_of_ne_0.
-Qed.
-Lemma natural_field_offset Γ τs i τ :
-  ✓ Γ → ✓{Γ}* τs → τs !! i = Some τ →
-  (natural_align_of Γ τ | field_offset Γ τs i).
-Proof.
-  intros ? Hτs. revert i. cut (∀ whole_align i pos, τs !! i = Some τ →
-    (default whole_align (head τs) (natural_align_of Γ) | pos) →
-    (natural_align_of Γ τ | pos + sum_list (take i
-       (natural_field_sizes (natural_size_of Γ) Γ whole_align pos τs)))).
-  { intros help i ?. rewrite <-(Nat.add_0_l (field_offset _ _ _)).
-    apply help; auto using Nat.divide_0_r. }
-  intros whole_align. induction Hτs as [|τ' τs Hτ Hτs IH];
-    intros [|i] pos al ?; simplify_equality'.
-  { rewrite Nat.add_0_r. auto using Nat.divide_0_r. }
-  rewrite Nat.add_assoc, (Nat.add_comm pos). apply IH; auto.
-  clear IH. destruct Hτs as [|τ2 τs]; simplify_list_equality.
-  rewrite <-Nat.add_assoc, (Nat.add_comm _ pos), Nat.add_assoc.
-  by apply natural_padding_divide, natural_align_ne_0.
+    by erewrite natural_field_sizes_weaken, natural_fields_align_weaken by eauto.
 Qed.
 End natural_type_environment.
