pointer_casts.v
@@ -22,10 +22,16 @@ Proof.
   | None => left _ | Some τ' => cast_if (decide (τ' = ucharT ∨ τ = τ'))
   end; abstract (try inversion 1; naive_solver constructor).
 Defined.
-Lemma castable_divide Γ τ τp : τ >*> τp → (ptr_size_of Γ τp | size_of Γ τ).
+Lemma size_of_castable Γ τ τp : τ >*> τp → (ptr_size_of Γ τp | size_of Γ τ).
+Proof. destruct 1; simpl; rewrite ?size_of_char; auto using Nat.divide_1_l. Qed.
+Lemma align_of_castable Γ τ1 τ2 :
+  ✓ Γ → τ1 >*> Some τ2 → (align_of Γ τ2 | align_of Γ τ1).
 Proof.
-  destruct 1; simpl; rewrite ?size_of_uchar; auto using Nat.divide_1_l.
+  inversion_clear 2; rewrite ?align_of_char; auto using Nat.divide_1_l.
 Qed.
+Lemma bit_align_of_castable Γ τ1 τ2 :
+  ✓ Γ → τ1 >*> Some τ2 → (bit_align_of Γ τ2 | bit_align_of Γ τ1).
+Proof. eauto using Nat.mul_divide_mono_r, align_of_castable. Qed.
 Lemma castable_type_valid Γ τ1 τ2 : ✓{Γ} τ1 → τ1 >*> Some τ2 → ✓{Γ} τ2.
 Proof. by inversion 2; subst; repeat constructor. Qed.
 Lemma castable_ptr_type_valid Γ τp1 τp2 : ✓{Γ} τp1 → τp1 >*> τp2 → ✓{Γ} τp2.
